src/mqtt-packet-parser/src/debug_ffi.c
@@ -1,0 +1,6 @@
+#include <stdio.h>
+#include <stdint.h>
+
+void print_hex(uint8_t i) {
+  printf("%02x", i);
+}
