src/mqtt-packet-parser/src/ffi.c
@@ -1,11 +1,5 @@
-#include <stdio.h>
 #include <stdint.h>
 #include "kremlib.h"
-
-// 本番環境では削除
-void print_hex(uint8_t i) {
-  printf("%02x", i);
-}
 
 C_String_t topic_name_uint8_to_c_string(uint8_t *u8_buffer) {
   return (char *)u8_buffer;
