src/mqtt-packet-parser/src/debug_ffi.fst
@@ -1,0 +1,9 @@
+module Debug_FFI
+
+module U8 = FStar.UInt8
+
+open FStar.HyperStack.ST
+
+assume val print_hex (i:U8.t): Stack unit
+  (requires (fun h -> true))
+  (ensures (fun h0 ret h1 -> true))
